Update Compil.lean

Leroy/Compil.lean
@@ -77,7 +77,7 @@ def machine_goes_wrong (C: List instr) (s_init: store) : Prop :=
    ∧ irred (transition C) (pc, stk, s)
    ∧ (instr_at C pc ≠ .some .Ihalt ∨ stk ≠ [])
 
-def compile_aexp (a: aexp) : List instr :=
+@[grind ]def compile_aexp (a: aexp) : List instr :=
   match a with
   | .CONST n => .Iconst n :: []
   | .VAR x => .Ivar x :: []
@@ -126,21 +126,21 @@ def compile_program (p: com) : List instr:=
 def smart_Ibranch (d: Int) : List instr:=
   if d = 0 then [] else .Ibranch d :: []
 
-@[grind] inductive code_at: List instr-> Int -> List instr-> Prop where
+@[grind] inductive code_at: List instr -> Int -> List instr-> Prop where
   | code_at_intro: forall C1 C2 C3 pc,
       pc = codelen C1 ->
       code_at (C1 ++ C2 ++ C3) pc C2
 
-theorem codelen_cons:
+@[grind] theorem codelen_cons:
   forall i c, codelen (i :: c) = codelen c + 1 := by grind
 
-theorem codelen_app:
+@[grind] theorem codelen_app:
   forall c1 c2, codelen (c1 ++ c2) = codelen c1 + codelen c2 := by
     intro c1 c2
     induction c1
     all_goals grind
 
-theorem instr_a : forall i c2 c1 pc,
+@[grind =>] theorem instr_a : forall i c2 c1 pc,
   pc = codelen c1 ->
   instr_at (c1.append (i :: c2) ) pc = .some i := by
     intro i c2 c1 pc
@@ -187,7 +187,7 @@ theorem code_at_head :
         dsimp
         grind
 
-theorem code_at_tail :
+@[grind] theorem code_at_tail :
    forall C pc i C',
   code_at C pc (i :: C') →
   code_at C (pc + 1) C' := by
@@ -199,7 +199,7 @@ theorem code_at_tail :
       apply code_at.code_at_intro
       grind
 
-theorem code_at_app_left:
+@[grind] theorem code_at_app_left:
   forall C pc C1 C2,
   code_at C pc (C1 ++ C2) ->
   code_at C pc C1 := by
@@ -209,7 +209,7 @@ theorem code_at_app_left:
       have := code_at.code_at_intro c1 m1 (m2 ++ c3) pc a
       grind [List.append_assoc]
 
-theorem code_at_app_right:
+@[grind] theorem code_at_app_right:
   forall C pc C1 C2,
   code_at C pc (C1 ++ C2) ->
   code_at C (pc + codelen C1) C2 := by
@@ -219,7 +219,7 @@ theorem code_at_app_right:
       have := code_at.code_at_intro (b ++ c1) c2 e (pc + codelen c1) (by grind)
       grind [List.append_assoc]
 
-theorem code_at_app_right2 : forall C pc C1 C2 C3,
+@[grind] theorem code_at_app_right2 : forall C pc C1 C2 C3,
   code_at C pc (C1 ++ C2 ++ C3) →
   code_at C (pc + codelen C1) C2 := by
     intro C pc c1 c2 c3 h
@@ -228,7 +228,7 @@ theorem code_at_app_right2 : forall C pc C1 C2 C3,
       have := code_at.code_at_intro (b ++ c1) c2 (c3 ++ e) (pc + codelen c1) (by grind)
       grind [List.append_assoc]
 
-theorem code_at_nil : forall C pc C1,
+@[grind] theorem code_at_nil : forall C pc C1,
   code_at C pc C1 -> code_at C pc [] := by
     intro C pc c1 h
     cases h
@@ -236,7 +236,7 @@ theorem code_at_nil : forall C pc C1,
       have := code_at.code_at_intro b [] (c1 ++ e) pc a
       grind [List.append_nil, List.append_assoc]
 
-theorem instr_at_code_at_nil :
+@[grind] theorem instr_at_code_at_nil :
   forall C pc i, instr_at C pc = .some i -> code_at C pc [] := by
     intro C pc i h
     induction C generalizing pc i
@@ -256,3 +256,669 @@ theorem instr_at_code_at_nil :
       next z =>
         have := code_at.code_at_intro [] [] (f :: t) pc
         grind [List.nil_append]
+
+theorem compile_aexp_correct (C : List instr) (s : store) (a : aexp) (pc : Int) (stk : stack) :
+  code_at C pc (compile_aexp a) →
+  transitions C (pc, stk, s) (pc + codelen (compile_aexp a), aeval s a :: stk, s) := by
+    induction a generalizing C pc stk
+    next =>
+      simp [aeval, compile_aexp]
+      intro a
+      unfold transitions
+      apply star_one
+      apply transition.trans_const
+      cases a
+      next => simp ; apply instr_a; grind
+    next =>
+      simp [aeval, compile_aexp]
+      intro a
+      apply star_one
+      apply transition.trans_var
+      cases a
+      next => simp ; apply instr_a; grind
+    next a1 a2 a1_ih a2_ih =>
+      simp [aeval, compile_aexp]
+      intro a
+      apply star_trans
+      . apply a1_ih
+        cases a
+        next c1 c3 a2 =>
+          have := code_at.code_at_intro c1 (compile_aexp a1) [instr.Iadd] pc a2
+          grind
+      . apply star_trans
+        . specialize a2_ih C (pc + codelen (compile_aexp a1)) (aeval s a1 :: stk)
+          apply a2_ih
+          cases a
+          next c1 c3 a =>
+            have := code_at.code_at_intro c1 (compile_aexp a2) (compile_aexp a2 ++ [instr.Iadd] ++ c3) pc a
+            grind
+        . apply star_one
+          cases a
+          next c1 c3 a =>
+            have h1 := instr_a instr.Iadd c3 (c1 ++ compile_aexp a1 ++ compile_aexp a2) (pc + codelen (compile_aexp a1) + codelen (compile_aexp a2)) (by grind)
+            have h2 := @transition.trans_add ((c1 ++ compile_aexp a1 ++ compile_aexp a2).append (instr.Iadd :: c3)) (pc + codelen (compile_aexp a1) + codelen (compile_aexp a2)) stk s (aeval s a1) (aeval s a2) (by grind)
+            simp [codelen_app, codelen_cons, codelen] at *
+            grind
+    next a1 a2 a1_ih a2_ih =>
+      simp [aeval, compile_aexp]
+      intro a
+      apply star_trans
+      . apply a1_ih
+        . cases a
+          next c1 c3 a =>
+            have := code_at.code_at_intro c1 (compile_aexp a1) ([instr.Iopp, instr.Iadd] ++ c3) pc a
+            grind [List.append_assoc, List.cons_append, List.nil_append]
+      . apply star_trans
+        . specialize a2_ih C (pc + codelen (compile_aexp a1)) (aeval s a1 :: stk)
+          apply a2_ih
+          cases a
+          next c1 c3 a =>
+            have := code_at.code_at_intro (c1 ++ (compile_aexp a1)) (compile_aexp a2) ([instr.Iopp, instr.Iadd] ++ c3)   (pc + codelen (compile_aexp a1)) (by grind)
+            grind
+        . apply star_trans
+          . apply star_one
+            have := @transition.trans_opp C (pc + codelen (compile_aexp a1) + codelen (compile_aexp a2)) ((aeval s a1) ::stk) s (aeval s a2)
+            apply this
+            cases a
+            next c1 c3 a =>
+              have := instr_a instr.Iopp (instr.Iadd :: c3) (c1 ++ compile_aexp a1 ++ compile_aexp a2) (pc + codelen (compile_aexp a1) + codelen (compile_aexp a2))
+              grind [List.append_assoc, List.cons_append, List.nil_append, List.append_eq]
+          . apply star_one
+            sorry
+
+
+
+
+
+
+
+
+
+
+
+
+
+
+
+
+
+
+
+
+
+
+
+
+
+
+
+
+-- - (* CONST *)
+--   apply star_one. apply trans_const. eauto with code.
+
+-- - (* VAR *)
+--   apply star_one. apply trans_var. eauto with code.
+
+-- - (* PLUS *)
+--   eapply star_trans. apply IHa1. eauto with code.
+--   eapply star_trans. apply IHa2. eauto with code.
+--   apply star_one. autorewrite with code. apply trans_add. eauto with code.
+
+-- - (* MINUS *)
+--   eapply star_trans. apply IHa1. eauto with code.
+--   eapply star_trans. apply IHa2. eauto with code.
+--   eapply star_trans.
+--   apply star_one. apply trans_opp. eauto with code.
+--   apply star_one.
+--   replace (aeval s a1 - aeval s a2)
+--      with (aeval s a1 + (- aeval s a2))
+--        by lia.
+--   autorewrite with code. apply trans_add. eauto with code.
+-- Qed.
+
+-- (** The proof for the compilation of Boolean expressions is similar.
+--   We recall the informal specification for the code generated by
+--   [compile_bexp b d1 d0]: it should
+-- - skip [d1] instructions if [b] evaluates to true,
+--        [d0] if [b] evaluates to false
+-- - leave the stack unchanged
+-- - leave the store unchanged.
+-- *)
+
+-- Lemma compile_bexp_correct:
+--   forall C s b d1 d0 pc stk,
+--   code_at C pc (compile_bexp b d1 d0) ->
+--   transitions C
+--        (pc, stk, s)
+--        (pc + codelen (compile_bexp b d1 d0) + (if beval s b then d1 else d0), stk, s).
+-- Proof.
+--   induction b; cbn; intros.
+
+-- - (* TRUE *)
+--   destruct (d1 =? 0) eqn:Z.
+--   + (* distance is zero, no branch is generated *)
+--     assert (d1 = 0) by (apply Z.eqb_eq; auto). subst d1.
+--     autorewrite with code. apply star_refl.
+--   + (* a branch is generated *)
+--     apply star_one. apply trans_branch with (d := d1). eauto with code. auto.
+
+-- - (* FALSE *)
+--   destruct (d0 =? 0) eqn:Z.
+--   + (* distance is zero, no branch is generated *)
+--     assert (d0 = 0) by (apply Z.eqb_eq; auto). subst d0.
+--     autorewrite with code. apply star_refl.
+--   + (* a branch is generated *)
+--     apply star_one. apply trans_branch with (d := d0). eauto with code. auto.
+
+-- - (* EQUAL *)
+--   eapply star_trans. apply compile_aexp_correct with (a := a1). eauto with code.
+--   eapply star_trans. apply compile_aexp_correct with (a := a2). eauto with code.
+--   apply star_one. apply trans_beq with (d1 := d1) (d0 := d0). eauto with code.
+--   autorewrite with code. auto.
+
+-- - (* LESSEQUAL *)
+--   eapply star_trans. apply compile_aexp_correct with (a := a1). eauto with code.
+--   eapply star_trans. apply compile_aexp_correct with (a := a2). eauto with code.
+--   apply star_one. apply trans_ble with (d1 := d1) (d0 := d0). eauto with code.
+--   autorewrite with code. auto.
+
+-- - (* NOT *)
+--   replace (if negb (beval s b) then d1 else d0)
+--      with (if beval s b then d0 else d1).
+--   apply IHb. auto.
+--   destruct (beval s b); auto.
+
+-- - (* AND *)
+--   set (code2 := compile_bexp b2 d1 d0) in *.
+--   set (code1 := compile_bexp b1 0 (codelen code2 + d0)) in *.
+--   eapply star_trans. apply IHb1. eauto with code.
+--   fold code1. destruct (beval s b1); cbn.
+--   + (* b1 evaluates to true, the code for b2 is executed *)
+--     autorewrite with code. apply IHb2. eauto with code.
+--   + (* b2 evaluates to true, the code for b2 is skipped *)
+--     autorewrite with code. apply star_refl.
+-- Qed.
+
+-- (** ** 4.2 Correctness of generated code for commands, terminating case. *)
+
+-- Lemma compile_com_correct_terminating:
+--   forall s c s',
+--   cexec s c s' ->
+--   forall C pc stk,
+--   code_at C pc (compile_com c) ->
+--   transitions C
+--       (pc, stk, s)
+--       (pc + codelen (compile_com c), stk, s').
+-- Proof.
+--   induction 1; cbn; intros.
+
+-- - (* SKIP *)
+--   autorewrite with code. apply star_refl.
+
+-- - (* ASSIGN *)
+--   eapply star_trans. apply compile_aexp_correct with (a := a). eauto with code.
+--   apply star_one. autorewrite with code. apply trans_setvar. eauto with code.
+
+-- - (* SEQUENCE *)
+--   eapply star_trans.
+--   apply IHcexec1. eauto with code.
+--   autorewrite with code. apply IHcexec2. eauto with code.
+
+-- - (* IFTHENELSE *)
+--   set (code1 := compile_com c1) in *.
+--   set (code2 := compile_com c2) in *.
+--   set (codeb := compile_bexp b 0 (codelen code1 + 1)) in *.
+--   eapply star_trans.
+--   apply compile_bexp_correct with (b := b). eauto with code.
+--   fold codeb. destruct (beval s b); autorewrite with code.
+--   + (* the "then" branch is selected *)
+--     eapply star_trans. apply IHcexec. eauto with code.
+--     fold code1. apply star_one. apply trans_branch with (d := codelen code2). eauto with code. lia.
+--   + (* then "else" branch is selected *)
+--     replace (pc + codelen codeb + codelen code1 + codelen code2 + 1)
+--        with (pc + codelen codeb + codelen code1 + 1 + codelen code2) by lia.
+--     apply IHcexec. eauto with code.
+
+-- - (* WHILE stop *)
+--   set (code_body := compile_com c) in *.
+--   set (code_branch := compile_bexp b 0 (codelen code_body + 1)) in *.
+--   set (d := - (codelen code_branch + codelen code_body + 1)) in *.
+--   eapply star_trans. apply compile_bexp_correct with (b := b). eauto with code.
+--   rewrite H. fold code_branch. autorewrite with code. apply star_refl.
+
+-- - (* WHILE loop *)
+--   set (code_body := compile_com c) in *.
+--   set (code_branch := compile_bexp b 0 (codelen code_body + 1)) in *.
+--   set (d := - (codelen code_branch + codelen code_body + 1)) in *.
+--   eapply star_trans. apply compile_bexp_correct with (b := b). eauto with code.
+--   rewrite H. fold code_branch. autorewrite with code.
+--   eapply star_trans. apply IHcexec1. eauto with code.
+--   eapply star_trans.
+--   apply star_one. apply trans_branch with (d := d). eauto with code. eauto.
+--   replace (pc + codelen code_branch + codelen code_body + 1 + d)
+--      with pc
+--        by lia.
+--   replace (pc + codelen code_branch + codelen code_body + 1)
+--      with (pc + codelen (compile_com (WHILE b c)))
+--        by (cbn; autorewrite with code; auto).
+--   apply IHcexec2. auto.
+-- Qed.
+
+-- (** As a corollary, we obtain the correctness of the compilation of whole
+--   programs, assuming they terminate. *)
+
+-- Theorem compile_program_correct_terminating:
+--   forall s c s',
+--   cexec s c s' ->
+--   machine_terminates (compile_program c) s s'.
+-- Proof.
+--   intros.
+--   set (C := compile_program c).
+--   assert (CODEAT: code_at C 0 (compile_com c ++ Ihalt :: nil)).
+--   { replace C with (nil ++ compile_program c ++ nil).
+--     apply code_at_intro. auto.
+--     rewrite app_nil_r; auto. }
+--   unfold machine_terminates.
+--   exists (0 + codelen (compile_com c)); split.
+-- - apply compile_com_correct_terminating. auto. eauto with code.
+-- - eauto with code.
+-- Qed.
+
+-- (** *** Exercise (2 stars, recommended). *)
+
+-- (** In a previous exercise, you modified [compile_com] to use
+--   [smart_Ibranch] instead of [Ibranch] so as to generate better code.
+--   Adapt the proof of [compile_com_correct_terminating] accordingly.
+--   Hint: first prove the following lemma, then use it! *)
+
+-- Lemma transitions_smart_Ibranch:
+--   forall C pc d pc' stk s,
+--   code_at C pc (smart_Ibranch d) ->
+--   pc' = pc + 1 + d ->
+--   transitions C (pc, stk, s) (pc', stk, s).
+-- Proof.
+--   unfold smart_Ibranch; intros.
+--   (* FILL IN HERE *)
+-- Abort.
+
+-- (** *** Exercise (4 stars, optional). *)
+
+-- (** Consider a loop with a simple test, such as [WHILE (LESSEQUAL a1 a2) c].
+--   Currently, the compiled code executes two branch instructions per iteration
+--   of the loop: one [Ible] to test the condition and one [Ibranch] to go back to
+--   the beginning of the loop.  We can reduce this to one [Ible] instruction
+--   per iteration, by putting the code for [c] before the code for the test:
+-- <<
+--      compile_com c ++ compile_bexp b delta1 0
+-- >>
+--   with [delta1] chosen so as to branch back to the beginning of [compile_com c]
+--   when [b] is true.
+
+--   By itself, this would compile while loops like do-while loops, which is
+--   incorrect.  On the first iteration, we must skip over the code for [c]
+--   and branch to the code that tests [b]:
+-- <<
+--     Ibranch (codesize(compile_com c)) :: compile_com c ++ compile_bexp b delta1 0
+-- >>
+--   In this exercise, you should modify [compile_com] to implement this
+--   alternate compilation schema for loops, then show its correctness
+--   by updating the statement and proof of [compile_com_correct_terminating].
+--   The difficulty (and the reason for the 4 stars) is that the hypothesis
+--   [code_at C pc (compile_com c)] no longer holds if [c] is a while loop
+--   and we are at the second iteration of the loop.  You need to come up
+--   with a more flexible way to relate the command [c] and the PC.
+-- *)
+
+-- (** * 7.  Full proof of compiler correctness *)
+
+-- (** We would like to strengthen the correctness result above so that it
+--   is not restricted to terminating source programs, but also applies to
+--   source program that diverge.  To this end, we abandon the big-step
+--   semantics for commands and switch to the small-step semantics with
+--   continuations.  We then show a simulation theorem, establishing that
+--   every transition of the small-step semantics in the source program
+--   is simulated (in a sense to be made precise below) by zero, one or
+--   several transitions of the machine executing the compiled code for
+--   the source program. *)
+
+-- (** Our first task is to relate configurations [(c, k, s)] of the small-step
+--   semantics with configurations [(C, pc, stk, s)] of the machine.
+--   We already know how to relate a command [c] with the machine code,
+--   using the [codeseq_at] predicate.  What needs to be defined is a relation
+--   between the continuation [k] and the machine code.
+
+--   Intuitively, when the machine finishes executing the generated code for
+--   command [c], that is, when it reaches the program point
+--   [pc + length(compile_com c)], the machine should continue by executing
+--   instructions that perform the pending computations described by
+--   continuation [k], then reach an [Ihalt] instruction to stop cleanly.
+
+--   We formalize this intution by the following inductive predicate
+--   [compile_cont C k pc], which states that, starting at program point [pc],
+--   there are instructions that perform the computations described in [k]
+--   and reach an [Ihalt] instruction. *)
+
+-- Inductive compile_cont (C: code): cont -> Z -> Prop :=
+--   | ccont_stop: forall pc,
+--       instr_at C pc = Some Ihalt ->
+--       compile_cont C Kstop pc
+--   | ccont_seq: forall c k pc pc',
+--       code_at C pc (compile_com c) ->
+--       pc' = pc + codelen (compile_com c) ->
+--       compile_cont C k pc' ->
+--       compile_cont C (Kseq c k) pc
+--   | ccont_while: forall b c k pc d pc' pc'',
+--       instr_at C pc = Some(Ibranch d) ->
+--       pc' = pc + 1 + d ->
+--       code_at C pc' (compile_com (WHILE b c)) ->
+--       pc'' = pc' + codelen (compile_com (WHILE b c)) ->
+--       compile_cont C k pc'' ->
+--       compile_cont C (Kwhile b c k) pc
+--   | ccont_branch: forall d k pc pc',
+--       instr_at C pc = Some(Ibranch d) ->
+--       pc' = pc + 1 + d ->
+--       compile_cont C k pc' ->
+--       compile_cont C k pc.
+
+-- (** Then, a configuration [(c,k,s)] of the small-step semantics matches
+--   a configuration [(C, pc, stk, s')] of the machine if the following conditions hold:
+-- - The stores are identical: [s' = s].
+-- - The machine stack is empty: [stk = nil].
+-- - The machine code at point [pc] is the compiled code for [c]:
+--   [code_at C pc (compile_com c)].
+-- - The machine code at point [pc + codelen (compile_com c)] matches continuation
+--   [k], in the sense of [compile_cont] above.
+-- *)
+
+-- Inductive match_config (C: code): com * cont * store -> config -> Prop :=
+--   | match_config_intro: forall c k st pc,
+--       code_at C pc (compile_com c) ->
+--       compile_cont C k (pc + codelen (compile_com c)) ->
+--       match_config C (c, k, st) (pc, nil, st).
+
+-- (** We are now ready to prove the expected simulation property.
+--   Since some transitions in the source command correspond to zero transitions
+--   in the compiled code, we need a simulation diagram of the "star" kind
+--   (see the slides).
+-- <<
+--                       match_config
+--      c / k / st  ----------------------- machconfig
+--        |                                   |
+--        |                                   | + or ( * and |c',k'| < |c,k} )
+--        |                                   |
+--        v                                   v
+--     c' / k' / st' ----------------------- machconfig'
+--                       match_config
+-- >>
+-- Note the stronger conclusion on the right:
+-- - either the virtual machine does one or several transitions
+-- - or it does zero, one or several transitions, but the size of the [c,k]
+--   pair decreases strictly.
+
+-- It would be equivalent to state:
+-- - either the virtual machine does one or several transitions
+-- - or it does zero transitions, but the size of the [c,k] pair decreases strictly.
+
+-- However, the formulation above, with the "star" case, is often more convenient.
+-- *)
+
+-- (** Finding an appropriate "anti-stuttering" measure is a bit of a black art.
+--   After trial and error, we find that the following measure works.  It is
+--   the sum of the sizes of the command [c] under focus and all the commands
+--   appearing in the continuation [k]. *)
+
+-- Fixpoint com_size (c: com) : nat :=
+--   match c with
+--   | SKIP => 1%nat
+--   | ASSIGN x a => 1%nat
+--   | (c1 ;; c2) => (com_size c1 + com_size c2 + 1)%nat
+--   | IFTHENELSE b c1 c2 => (com_size c1 + com_size c2 + 1)%nat
+--   | WHILE b c1 => (com_size c1 + 1)%nat
+--   end.
+
+-- Remark com_size_nonzero: forall c, (com_size c > 0)%nat.
+-- Proof.
+--   induction c; cbn; lia.
+-- Qed.
+
+-- Fixpoint cont_size (k: cont) : nat :=
+--   match k with
+--   | Kstop => 0%nat
+--   | Kseq c k' => (com_size c + cont_size k')%nat
+--   | Kwhile b c k' => cont_size k'
+--   end.
+
+-- Definition measure (impconf: com * cont * store) : nat :=
+--   match impconf with (c, k, m) => (com_size c + cont_size k)%nat end.
+
+-- (** A few technical lemmas to help with the simulation proof. *)
+
+-- Lemma compile_cont_Kstop_inv:
+--   forall C pc s,
+--   compile_cont C Kstop pc ->
+--   exists pc',
+--   star (transition C) (pc, nil, s) (pc', nil, s)
+--   /\ instr_at C pc' = Some Ihalt.
+-- Proof.
+--   intros. dependent induction H.
+-- - exists pc; split. apply star_refl. auto.
+-- - destruct IHcompile_cont as (pc'' & A & B); auto.
+--   exists pc''; split; auto. eapply star_step; eauto. eapply trans_branch; eauto.
+-- Qed.
+
+-- Lemma compile_cont_Kseq_inv:
+--   forall C c k pc s,
+--   compile_cont C (Kseq c k) pc ->
+--   exists pc',
+--   star (transition C) (pc, nil, s) (pc', nil, s)
+--   /\ code_at C pc' (compile_com c)
+--   /\ compile_cont C k (pc' + codelen(compile_com c)).
+-- Proof.
+--   intros. dependent induction H.
+-- - exists pc; split. apply star_refl. split; congruence.
+-- - edestruct IHcompile_cont as (pc'' & A & B). eauto.
+--   exists pc''; split; auto. eapply star_step; eauto. eapply trans_branch; eauto.
+-- Qed.
+
+-- Lemma compile_cont_Kwhile_inv:
+--   forall C b c k pc s,
+--   compile_cont C (Kwhile b c k) pc ->
+--   exists pc',
+--   plus (transition C) (pc, nil, s) (pc', nil, s)
+--   /\ code_at C pc' (compile_com (WHILE b c))
+--   /\ compile_cont C k (pc' + codelen(compile_com (WHILE b c))).
+-- Proof.
+--   intros. dependent induction H.
+-- - exists (pc + 1 + d); split.
+--   apply plus_one. eapply trans_branch; eauto.
+--   split; congruence.
+-- - edestruct IHcompile_cont as (pc'' & A & B & D). eauto.
+--   exists pc''; split; auto. eapply plus_left. eapply trans_branch; eauto. apply plus_star; auto.
+-- Qed.
+
+-- Lemma match_config_skip:
+--   forall C k s pc,
+--   compile_cont C k pc ->
+--   match_config C (SKIP, k, s) (pc, nil, s).
+-- Proof.
+--   intros. constructor.
+-- - cbn. inversion H; eauto with code.
+-- - cbn. autorewrite with code. auto.
+-- Qed.
+
+-- (** At last, we can state and prove the simulation diagram. *)
+
+-- Lemma simulation_step:
+--   forall C impconf1 impconf2 machconf1,
+--   step impconf1 impconf2 ->
+--   match_config C impconf1 machconf1 ->
+--   exists machconf2,
+--       (plus (transition C) machconf1 machconf2
+--        \/ (star (transition C) machconf1 machconf2
+--            /\ (measure impconf2 < measure impconf1)%nat))
+--    /\ match_config C impconf2 machconf2.
+-- Proof.
+--   intros until machconf1; intros STEP MATCH.
+--   inversion STEP; clear STEP; subst; inversion MATCH; clear MATCH; subst; cbn in *.
+
+-- - (* assign *)
+--   econstructor; split.
+--   left. eapply plus_right. eapply compile_aexp_correct; eauto with code.
+--   eapply trans_setvar; eauto with code.
+--   autorewrite with code in *. apply match_config_skip. auto.
+
+-- - (* seq *)
+--   econstructor; split.
+--   right; split. apply star_refl. lia.
+--   autorewrite with code in *. constructor. eauto with code. eapply ccont_seq; eauto with code.
+
+-- - (* if *)
+--   set (code1 := compile_com c1) in *.
+--   set (codeb := compile_bexp b 0 (codelen code1 + 1)) in *.
+--   set (code2 := compile_com c2) in *.
+--   autorewrite with code in *.
+--   econstructor; split.
+--   right; split.
+--   apply compile_bexp_correct with (b := b). eauto with code.
+--   destruct (beval s b); lia.
+--   fold codeb. destruct (beval s b).
+--   + autorewrite with code. constructor. eauto with code.
+--     eapply ccont_branch. eauto with code. eauto.
+--     fold code1.
+--     replace (pc + codelen codeb + codelen code1 + 1 + codelen code2)
+--        with (pc + codelen codeb + codelen code1 + codelen code2 + 1) by lia.
+--     auto.
+--   + autorewrite with code. constructor. eauto with code. auto.
+--     fold code2.
+--     replace (pc + codelen codeb + codelen code1 + 1 + codelen code2)
+--        with (pc + codelen codeb + codelen code1 + codelen code2 + 1) by lia.
+--     auto.
+
+-- - (* while stop *)
+--   set (codec := compile_com c) in *.
+--   set (codeb := compile_bexp b 0 (codelen codec + 1)) in *.
+--   econstructor; split.
+--   right; split.
+--   apply compile_bexp_correct with (b := b). eauto with code.
+--   assert (com_size c > 0)%nat by apply com_size_nonzero. lia.
+--   rewrite H. fold codeb. autorewrite with code in *. apply match_config_skip. auto.
+
+-- - (* while loop *)
+--   set (codec := compile_com c) in *.
+--   set (codeb := compile_bexp b 0 (codelen codec + 1)) in *.
+--   econstructor; split.
+--   right; split.
+--   apply compile_bexp_correct with (b := b). eauto with code.
+--   lia.
+--   rewrite H. fold codeb. autorewrite with code in *.
+--   constructor. eauto with code.
+--   eapply ccont_while with (pc' := pc). eauto with code. fold codec. lia.
+--   auto.
+--   cbn. fold codec; fold codeb. eauto.
+--   autorewrite with code. auto.
+
+-- - (* skip seq *)
+--   autorewrite with code in *.
+--   edestruct compile_cont_Kseq_inv as (pc' & X & Y & Z). eauto.
+--   econstructor; split.
+--   right; split. eauto. lia.
+--   constructor; auto.
+
+-- - (* skip while *)
+--   autorewrite with code in *.
+--   edestruct compile_cont_Kwhile_inv as (pc' & X & Y & Z). eauto.
+--   econstructor; split.
+--   left. eauto.
+--   constructor; auto.
+-- Qed.
+
+-- (** The hard work is done!  Nice consequences will follow. *)
+
+-- (** First, we get an alternate proof of [compile_program_correct_terminating],
+--   using the continuation semantics instead of the big-step semantics
+--   to characterize termination of the source program. *)
+
+-- Lemma simulation_steps:
+--   forall C impconf1 impconf2, star step impconf1 impconf2 ->
+--   forall machconf1, match_config C impconf1 machconf1 ->
+--   exists machconf2,
+--      star (transition C) machconf1 machconf2
+--   /\ match_config C impconf2 machconf2.
+-- Proof.
+--   induction 1; intros.
+-- - exists machconf1; split; auto. apply star_refl.
+-- - edestruct simulation_step as (machconf2 & STEPS2 & MATCH2); eauto.
+--   edestruct IHstar as (machconf3 & STEPS3 & MATCH3); eauto.
+--   exists machconf3; split; auto.
+--   eapply star_trans; eauto.
+--   destruct STEPS2 as [A | [A B]]. apply plus_star; auto. auto.
+-- Qed.
+
+-- Lemma match_initial_configs:
+--   forall c s,
+--   match_config (compile_program c) (c, Kstop, s) (0, nil, s).
+-- Proof.
+--   intros. set (C := compile_program c).
+--   assert (code_at C 0 (compile_com c ++ Ihalt :: nil)).
+--   { replace C with (nil ++ (compile_com c ++ Ihalt :: nil) ++ nil).
+--     constructor; auto.
+--     rewrite app_nil_r; auto. }
+--   constructor.
+-- - eauto with code.
+-- - apply ccont_stop. eauto with code.
+-- Qed.
+
+-- Theorem compile_program_correct_terminating_2:
+--   forall c s s',
+--   star step (c, Kstop, s) (SKIP, Kstop, s') ->
+--   machine_terminates (compile_program c) s s'.
+-- Proof.
+--   intros. set (C := compile_program c).
+--   edestruct (simulation_steps C) as (ms & A & B). eauto. apply match_initial_configs.
+--   inversion B; subst.
+--   edestruct compile_cont_Kstop_inv as (pc' & D & E). eauto.
+--   exists pc'; split; auto.
+--   eapply star_trans. eauto. cbn in D; autorewrite with code in D. eauto.
+-- Qed.
+
+-- (** Second, and more importantly, we get a proof of semantic preservation
+--   for diverging source programs: if the program makes infinitely many steps,
+--   the generated code makes infinitely many machine transitions. *)
+
+-- Lemma simulation_infseq_inv:
+--   forall C n impconf1 machconf1,
+--   infseq step impconf1 -> match_config C impconf1 machconf1 ->
+--   (measure impconf1 < n)%nat ->
+--   exists impconf2 machconf2,
+--       infseq step impconf2
+--    /\ plus (transition C) machconf1 machconf2
+--    /\ match_config C impconf2 machconf2.
+-- Proof.
+--   induction n; intros impconf1 machconf1 INFSEQ MATCH MEASURE.
+-- - exfalso; lia.
+-- - inversion INFSEQ; clear INFSEQ; subst.
+--   edestruct simulation_step as (machconf2 & [PLUS | [STAR LESS]] & MATCH2). eauto. eauto.
+-- + exists b, machconf2; auto.
+-- + edestruct IHn as (impconf3 & machconf3 & X & Y & Z). eauto. eauto. lia.
+--   exists impconf3, machconf3.
+--   split. auto.
+--   split. eapply star_plus_trans; eauto.
+--   auto.
+-- Qed.
+
+-- Theorem compile_program_correct_diverging:
+--   forall c s,
+--   infseq step (c, Kstop, s) ->
+--   machine_diverges (compile_program c) s.
+-- Proof.
+--   intros. set (C := compile_program c).
+--   apply infseq_coinduction_principle_2 with
+--     (X := fun machconf =>
+--           exists impconf, infseq step impconf /\ match_config C impconf machconf).
+-- - intros machconf (impconf & INFSEQ & MATCH).
+--   edestruct (simulation_infseq_inv C (S (measure impconf)))
+--   as (impconf2 & machconf2 & INFSEQ2 & PLUS & MATCH2).
+--   eauto. eauto. lia.
+--   exists machconf2; split. auto. exists impconf2; auto.
+-- - exists (c, Kstop, s); split. auto. apply match_initial_configs.
+-- Qed.
